revert reorder to list format, polish
revert reordering input format to `nat option list` (was `nat => nat option`). somewhat simpler proofs in some parts, but usage (see `tape_offset` and relevant proofs) is significantly easier and straightforward

papers/116_stefan_rass/TM.thy
@@ -509,96 +509,104 @@ corollary wf_steps[intro]: "wf_config c \<Longrightarrow> wf_config (steps n c)"
 
 end \<comment> \<open>\<^locale>\<open>TM\<close>\<close>
 
+
+subsection\<open>TM Modifications\<close>
+
 subsubsection\<open>Reordering Tapes\<close>
 
+(* TODO document this section *)
 
-definition reorder :: "(nat \<Rightarrow> nat option) \<Rightarrow> 'a list \<Rightarrow> 'a list \<Rightarrow> 'a list"
-  where "reorder p xs ys = map2 (\<lambda>i x. case p i of None \<Rightarrow> x | Some i' \<Rightarrow> nth_or i' x ys) [0..<length xs] xs"
+definition reorder :: "(nat option list) \<Rightarrow> 'a list \<Rightarrow> 'a list \<Rightarrow> 'a list"
+  where "reorder is xs ys = map2 (\<lambda>i x. case is ! i of None \<Rightarrow> x | Some i' \<Rightarrow> nth_or i' x ys) [0..<length xs] xs"
 
-value "reorder (\<lambda>i. [Some 0, Some 2, Some 1, None]!i) (x\<up>4) [a,b,c]"
+value "reorder [Some 0, Some 2, Some 1, None] [w,x,y,z] [a,b,c]"
 
-lemma reorder_length[simp]: "length (reorder p xs ys) = length xs" unfolding reorder_def by simp
+lemma reorder_length[simp]: "length (reorder is xs ys) = length xs" unfolding reorder_def by simp
 
-lemma reorder_Nil[simp]: "reorder p xs [] = xs"
+lemma reorder_Nil[simp]: "reorder is xs [] = xs"
   unfolding reorder_def nth_or_Nil case_option_same prod.snd_def[symmetric] by simp
 
 lemma reorder_nth[simp]:
   assumes "i < length xs"
-  shows "reorder p xs ys ! i = (case p i of None \<Rightarrow> xs ! i | Some i' \<Rightarrow> nth_or i' (xs ! i) ys)"
+  shows "reorder is xs ys ! i = (case is ! i of None \<Rightarrow> xs ! i | Some i' \<Rightarrow> nth_or i' (xs ! i) ys)"
   using assms unfolding reorder_def by (subst nth_map2) auto
 
-lemma reorder_map[simp]: "map f (reorder p xs ys) = reorder p (map f xs) (map f ys)"
+lemma reorder_map[simp]: "map f (reorder is xs ys) = reorder is (map f xs) (map f ys)"
 proof -
-  have "map f (reorder p xs ys) = map (\<lambda>(i, x). f (case p i of None \<Rightarrow> x | Some i' \<Rightarrow> nth_or i' x ys)) (zip [0..<length xs] xs)"
+  let ?m = "\<lambda>d i x. case is ! i of None \<Rightarrow> d x | Some i' \<Rightarrow> nth_or i' (d x) (map f ys)"
+  let ?m' = "\<lambda>d (i, x). ?m d i x" and ?id = "\<lambda>x. x"
+  have "map f (reorder is xs ys) =
+    map (\<lambda>(i, x). f (case is ! i of None \<Rightarrow> x | Some i' \<Rightarrow> nth_or i' x ys)) (zip [0..<length xs] xs)"
     unfolding reorder_def map_map comp_def by force
-  also have "... = map2 (\<lambda>i x. case p i of None \<Rightarrow> f x | Some i' \<Rightarrow> nth_or i' (f x) (map f ys)) [0..<length xs] xs"
-    unfolding option.case_distrib nth_or_map ..
-  also have "... = map ((\<lambda>(i, x). case p i of None \<Rightarrow> x | Some i' \<Rightarrow> nth_or i' x (map f ys)) \<circ> (\<lambda>(i, x). (i, f x))) (zip [0..<length xs] xs)"
-    by fastforce
-  also have "... = map (\<lambda>(i, x). case p i of None \<Rightarrow> x | Some i' \<Rightarrow> nth_or i' x (map f ys)) (map (\<lambda>(i, x). (i, f x)) (zip [0..<length xs] xs))"
-    by force
-  also have "... = map2 (\<lambda>i x. case p i of None \<Rightarrow> x | Some i' \<Rightarrow> nth_or i' x (map f ys)) [0..<length xs] (map f xs)"
+  also have "... = map2 (?m f) [0..<length xs] xs" unfolding option.case_distrib nth_or_map ..
+  also have "... = map ((?m' ?id) \<circ> (\<lambda>(i, x). (i, f x))) (zip [0..<length xs] xs)" by fastforce
+  also have "... = map (?m' ?id) (map (\<lambda>(i, x). (i, f x)) (zip [0..<length xs] xs))" by force
+  also have "... = map2 (?m ?id) [0..<length xs] (map f xs)"
     unfolding zip_map_map[symmetric] list.map_ident ..
-  also have "... = reorder p (map f xs) (map f ys)" unfolding reorder_def by simp
+  also have "... = reorder is (map f xs) (map f ys)" unfolding reorder_def by simp
   finally show ?thesis .
 qed
 
 
 (* TODO are both xs and ys needed here? in practice they seem always be identical *)
-definition reorder_inv :: "(nat \<Rightarrow> nat option) \<Rightarrow> 'a list \<Rightarrow> 'a list"
-  where "reorder_inv p ys = map
-    (\<lambda>i. ys ! (LEAST i'. i'<length ys \<and> p i' = Some i))
-    [0..<Suc (Max (Option.these (p ` {0..<length ys})))]"
+definition reorder_inv :: "(nat option list) \<Rightarrow> 'a list \<Rightarrow> 'a list"
+  where "reorder_inv is ys = map
+    (\<lambda>i. ys ! (LEAST i'. i'<length is \<and> is ! i' = Some i))
+    [0..<if set is \<subseteq> {None} then 0 else Suc (Max (Option.these (set is)))]"
 
 
-lemma card_these_helper: "card (Option.these (f ` {0..<n})) \<le> n"
+lemma card_these_helper: "card (Option.these (set xs)) \<le> length xs"
 proof -
-  have "card (Option.these (f ` {0..<n})) \<le> card (f ` {0..<n})" by (rule card_these) blast
-  also have "... \<le> card {0..<n}" by (rule card_image_le) blast
-  also have "... \<le> n" by simp
+  have "card (Option.these (set xs)) \<le> card (set xs)" by (rule card_these) blast
+  also have "... \<le> length xs" by (rule card_length)
   finally show ?thesis .
 qed
 
 lemma reorder_inv:
-  assumes "ys \<noteq> []"
-    and items_match: "Option.these (p ` {0..<length xs}) = {0..<length ys}"
-  shows "reorder_inv p (reorder p xs ys) = ys"
+  assumes [simp]: "length xs = length is"
+    and items_match: "Option.these (set is) = {0..<length ys}"
+  shows "reorder_inv is (reorder is xs ys) = ys"
 proof -
-  from \<open>ys \<noteq> []\<close> have "length ys > 0" by simp
 
-  define zs where "zs \<equiv> reorder p xs ys"
+  define zs where "zs \<equiv> reorder is xs ys"
   have lz: "length zs = length xs" unfolding zs_def reorder_length ..
 
-  from \<open>length ys > 0\<close>have *:
-    "Suc (Max (Option.these (p ` {0..<length xs}))) = length ys"
-    unfolding items_match Max_atLeastLessThan_nat[OF \<open>length ys > 0\<close>] by auto
+  have *: "(if set is \<subseteq> {None} then 0 else Suc (Max (Option.these (set is)))) = length ys"
+  proof (rule ifI)
+    assume "set is \<subseteq> {None}"
+    then have "Option.these (set is) = {}" unfolding these_empty_eq subset_singleton_iff .
+    then have "{0..<length ys} = {}" unfolding items_match .
+    then show "0 = length ys" by simp
+  next
+    assume "\<not> set is \<subseteq> {None}"
+    then have "Option.these (set is) \<noteq> {}" unfolding these_empty_eq subset_singleton_iff .
+    then have "0 < length ys" unfolding items_match by simp
+    then show "Suc (Max (Option.these (set is))) = length ys"
+      unfolding items_match Max_atLeastLessThan_nat[OF \<open>length ys > 0\<close>] by simp
+  qed
 
-  have "length ys = card (Option.these (p ` {0..<length xs}))" unfolding items_match by simp
-  also have "... \<le> length xs" by (rule card_these_helper)
-  finally have ls: "length xs \<ge> length ys" .
-  then have mls: "min (length [0..<length ys]) (length xs) = length ys" by simp
+  have "length ys = card (Option.these (set is))" unfolding items_match by simp
+  also have "... \<le> length is" by (rule card_these_helper)
+  finally have ls: "length is \<ge> length ys" .
 
-  have "reorder_inv p (reorder p xs ys) = map ((!) ys) [0..<length ys]"
+  have "reorder_inv is (reorder is xs ys) = map ((!) ys) [0..<length ys]"
     unfolding reorder_inv_def zs_def[symmetric] lz *
   proof (intro list.map_cong0)
     fix n assume "n \<in> set [0..<length ys]"
     then have [simp]: "n < length ys" by simp
     then have *: "[0..<length ys] ! n = n" by simp
 
-    define i where "i = (LEAST i. i < length xs \<and> p i = Some n)"
+    define i where "i = (LEAST i. i < length is \<and> is ! i = Some n)"
 
-    from \<open>n < length ys\<close> have "n \<in> Option.these (p ` {0..<length xs})" unfolding items_match by simp
-    then have "Some n \<in> p ` {0..<length xs}" unfolding these_altdef by force
-    then have [simp]: "\<exists>i. i < length xs \<and> p i = Some n" unfolding image_iff by fastforce
+    from \<open>n < length ys\<close> have "n \<in> Option.these (set is)" unfolding items_match by simp
+    then have "Some n \<in> set is" unfolding these_altdef by force
+    then have ex_i[simp]: "\<exists>i. i < length is \<and> is ! i = Some n" unfolding in_set_conv_nth .
 
-    then have "i < length xs \<and> p i = Some n" unfolding i_def by (rule LeastI_ex)
-    then have [simp]: "i < length xs" and [simp]: "p i = Some n" by blast+
-    then have [simp]: "[0..<length xs] ! i = i" by simp
+    then have "i < length is \<and> is ! i = Some n" unfolding i_def by (rule LeastI_ex)
+    then have [simp]: "i < length is" and [simp]: "is ! i = Some n" by blast+
+    then have [simp]: "[0..<length is] ! i = i" by simp
 
-    have **: "nth_or i x (map2 (\<lambda>x y. case p x of None \<Rightarrow> y | Some i' \<Rightarrow> nth_or i' y ys) [0..<length xs] xs)
-        = ys ! n" for x by simp
-
-    show "zs ! (LEAST i'. i' < length xs \<and> p i' = Some n) = ys ! n"
+    show "zs ! (LEAST i'. i' < length is \<and> is ! i' = Some n) = ys ! n"
       unfolding i_def[symmetric] zs_def reorder_def by simp
   qed
   then show ?thesis unfolding map_nth .
@@ -607,55 +615,55 @@ qed
 (* definition reorder_fun *)
   (* where "reorder_fun f k l = map (\<lambda>i. if i \<in> f ` {0..<l} then Some (inv_into {0..<l} f i) else None) [0..<k]" *)
 
-definition reorder_config :: "(nat \<Rightarrow> nat option) \<Rightarrow> 's tape list \<Rightarrow> ('q, 's) TM_config \<Rightarrow> ('q, 's) TM_config"
-  where "reorder_config p tps c = \<lparr> state = state c, tapes = reorder p tps (tapes c) \<rparr>"
+definition reorder_config :: "(nat option list) \<Rightarrow> 's tape list \<Rightarrow> ('q, 's) TM_config \<Rightarrow> ('q, 's) TM_config"
+  where "reorder_config is tps c = \<lparr> state = state c, tapes = reorder is tps (tapes c) \<rparr>"
 
 lemma reorder_config_length[simp]: "length (tapes (reorder_config p tps c)) = length tps"
   unfolding reorder_config_def TM_config.simps reorder_length ..
 
 lemma reorder_config_simps[simp]:
-  shows reorder_config_state: "state (reorder_config p tps c) = state c"
-    and reorder_config_tapes: "tapes (reorder_config p tps c) = reorder p tps (tapes c)"
+  shows reorder_config_state: "state (reorder_config is tps c) = state c"
+    and reorder_config_tapes: "tapes (reorder_config is tps c) = reorder is tps (tapes c)"
   unfolding reorder_config_def by simp_all
 
 
-locale reorder_tapes =
+locale TM_reorder_tapes =
   fixes M :: "('q, 's::finite) TM"
-    and p :: "nat \<Rightarrow> nat option"
-    and k' :: nat
-  assumes items_match: "Option.these (p ` {0..<k'}) = {0..<TM.tape_count M}"
+    and "is" :: "nat option list"
+  assumes items_match: "Option.these (set is) = {0..<TM.tape_count M}"
 begin
 sublocale TM .
+
+abbreviation "k' \<equiv> length is"
 
 lemma k_k': "k \<le> k'"
 proof -
   have "k = card {0..<k}" by simp
-  also have "... = card (Option.these (p ` {0..<k'}))" unfolding items_match ..
-  also have "... \<le> card (p ` {0..<k'})" by (rule card_these) blast
-  also have "... \<le> card {0..<k'}" by (rule card_image_le) blast
-  also have "... = k'" by simp
+  also have "... = card (Option.these (set is))" unfolding items_match ..
+  also have "... \<le> card (set is)" by (rule card_these) blast
+  also have "... \<le> k'" by (rule card_length)
   finally show "k \<le> k'" .
 qed
 
 definition reorder_tapes_rec :: "('q, 's) TM_record"
   where "reorder_tapes_rec \<equiv>
-    let h = reorder_inv p in
+    let h = reorder_inv is in
     M_rec \<lparr>
       tape_count := k',
       next_state := \<lambda>q hds. \<delta>\<^sub>q q (h hds),
-      next_write := \<lambda>q hds i. case p i of Some i \<Rightarrow> (\<delta>\<^sub>w q (h hds) i) | None \<Rightarrow> hds ! i,
-      next_move  := \<lambda>q hds i. case p i of Some i \<Rightarrow> (\<delta>\<^sub>m q (h hds) i) | None \<Rightarrow> No_Shift
+      next_write := \<lambda>q hds i. case is ! i of Some i \<Rightarrow> (\<delta>\<^sub>w q (h hds) i) | None \<Rightarrow> hds ! i,
+      next_move  := \<lambda>q hds i. case is ! i of Some i \<Rightarrow> (\<delta>\<^sub>m q (h hds) i) | None \<Rightarrow> No_Shift
     \<rparr>"
 
 lemma reorder_tapes_rec_simps: "reorder_tapes_rec = \<lparr>
   TM_record.tape_count = k',
   states = Q, initial_state = q\<^sub>0, final_states = F, accepting_states = F\<^sup>+,
-  next_state = \<lambda>q hds. \<delta>\<^sub>q q (reorder_inv p hds),
-  next_write = \<lambda>q hds i. case p i of Some i \<Rightarrow> (\<delta>\<^sub>w q (reorder_inv p hds) i) | None \<Rightarrow> hds ! i,
-  next_move  = \<lambda>q hds i. case p i of Some i \<Rightarrow> (\<delta>\<^sub>m q (reorder_inv p hds) i) | None \<Rightarrow> No_Shift
+  next_state = \<lambda>q hds. \<delta>\<^sub>q q (reorder_inv is hds),
+  next_write = \<lambda>q hds i. case is ! i of Some i \<Rightarrow> (\<delta>\<^sub>w q (reorder_inv is hds) i) | None \<Rightarrow> hds ! i,
+  next_move  = \<lambda>q hds i. case is ! i of Some i \<Rightarrow> (\<delta>\<^sub>m q (reorder_inv is hds) i) | None \<Rightarrow> No_Shift
 \<rparr>" unfolding reorder_tapes_rec_def Let_def by simp
 
-definition [simp]: "M' \<equiv> Abs_TM reorder_tapes_rec"
+definition "M' \<equiv> Abs_TM reorder_tapes_rec"
 
 lemma M'_valid: "is_valid_TM reorder_tapes_rec"
   unfolding reorder_tapes_rec_simps
@@ -665,16 +673,16 @@ qed (fact state_axioms)+
 
 sublocale M': TM M' .
 
-lemma M'_rec: "M'.M_rec = reorder_tapes_rec" using Abs_TM_inverse M'_valid by auto
+lemma M'_rec: "M'.M_rec = reorder_tapes_rec" using Abs_TM_inverse M'_valid by (auto simp add: M'_def)
 lemmas M'_simps = M'.TM_fields_defs M'_rec reorder_tapes_rec_simps TM_record.simps
 
 lemma M'_F: "M'.F = F" unfolding M'_simps ..
-lemma M'_k: "M'.k = k'" unfolding M'_simps ..
+lemma M'_k[simp]: "M'.k = k'" unfolding M'_simps ..
 
-lemma reorder_steps:
+lemma reorder_step:
   assumes "wf_config c"
     and "M'.wf_config c'"
-  shows "M'.step (reorder_config p (tapes c') c) = reorder_config p (tapes c') (step c)"
+  shows "M'.step (reorder_config is (tapes c') c) = reorder_config is (tapes c') (step c)"
     (is "M'.step (?rc c) = ?rc (step c)")
 proof (cases "is_final c")
   assume "is_final c"
@@ -687,19 +695,16 @@ next
   let ?q = "state c" and ?q' = "state ?c'"
   let ?tps = "tapes c" and ?hds = "heads c"
 
-  let ?r = "reorder p"
+  let ?r = "reorder is"
   let ?hds' = "?r (heads c') ?hds" and ?tps' = "?r (tapes c') ?tps"
 
   from \<open>wf_config c\<close> have l_tps: "length (tapes c) = k" by simp
   then have l_hds: "length (heads c) = k" by simp
-  from \<open>M'.wf_config c'\<close> have l_tps': "length (tapes c') = k'" unfolding TM.wf_config_def M'_k .
+  from \<open>M'.wf_config c'\<close> have l_tps': "length (tapes c') = k'" by simp
   then have l_hds': "length (heads c') = k'" by simp
 
-  (* have l_hds'': "length ?hds' = k'" unfolding reorder_length l_hds' M'_k .. *)
-  from at_least_one_tape have "?hds \<noteq> []" unfolding length_0_conv[symmetric] l_hds by simp
-  moreover have "Option.these (p ` {0..<length (heads c')}) = {0..<length ?hds}"
-    unfolding l_hds l_hds' unfolding items_match ..
-  ultimately have r_inv_hds[simp]: "reorder_inv p (reorder p (heads c') ?hds) = ?hds" by (rule reorder_inv)
+  moreover have "Option.these (set is) = {0..<length ?hds}" unfolding l_hds unfolding items_match ..
+  ultimately have r_inv_hds[simp]: "reorder_inv is (reorder is (heads c') ?hds) = ?hds" by (rule reorder_inv)
 
   assume "\<not> is_final c"
   then have "\<not> M'.is_final ?c'" unfolding M'_F by simp
@@ -713,26 +718,25 @@ next
       unfolding step_not_final_def Let_def by simp
     finally show "state (M'.step_not_final ?c') = state (?rc (step_not_final c))" .
 
-    from k_k' have min_k_k': "min k M'.k = k" unfolding M'_k by simp
-    have lr: "length (reorder p (tapes c') x) = M'.k" for x unfolding reorder_length l_tps' M'_k ..
+    from k_k' have min_k_k': "min k M'.k = k" by simp
+    have lr: "length (reorder is (tapes c') x) = M'.k" for x unfolding reorder_length l_tps' M'_k ..
 
     have "tapes (M'.step_not_final ?c') = map2 tape_action (M'.\<delta>\<^sub>a ?q ?hds') ?tps'"
       unfolding M'.step_not_final_def by (simp add: Let_def)
     also have "... = ?r (tapes c') (map2 tape_action (\<delta>\<^sub>a ?q ?hds) ?tps)"
     proof (rule M'.step_not_final_eqI)
       thm reorder_length
-      let ?r = "reorder p"
+      let ?r = "reorder is"
       let ?rt = "?r (tapes c')"
       fix i assume "i < M'.k"
       then have [simp]: "i < k'" unfolding M'_k .
-      (* then have [simp]: "nth_or i x is = is ! i" for x by simp *)
 
       show "tape_action (M'.\<delta>\<^sub>w ?q ?hds' i, M'.\<delta>\<^sub>m ?q ?hds' i) (?tps' ! i) =
         ?rt (map2 tape_action (\<delta>\<^sub>a ?q ?hds) ?tps) ! i"
-      proof (induction "p i")
+      proof (induction "is ! i")
         case None
-        then have [simp]: "p i = None" ..
-        from \<open>i < k'\<close> have "reorder p xs ys ! i = xs ! i" if "length xs = k'" for xs ys :: "'x list"
+        then have [simp]: "is ! i = None" ..
+        from \<open>i < k'\<close> have "reorder is xs ys ! i = xs ! i" if "length xs = k'" for xs ys :: "'x list"
           using that by simp
         note * = this[OF l_tps'] this[OF l_hds']
         from \<open>i < k'\<close> have [simp]: "map head (tapes c') ! i = head (tapes c' ! i)"
@@ -740,18 +744,17 @@ next
         show ?case unfolding M'_simps * by simp
       next
         case (Some i')
-        then have [simp]: "p i = Some i'" ..
-
+        then have [simp]: "is ! i = Some i'" ..
 
         from \<open>i < k'\<close> have "i \<in> {0..<k'}" by simp
-        then have "Some i' \<in> p ` {0..<k'}" unfolding \<open>Some i' = p i\<close> by blast
+        then have "Some i' \<in> set is" unfolding \<open>Some i' = is ! i\<close> using \<open>i < k'\<close> nth_mem by blast
         then have "i' \<in> {0..<k}" unfolding items_match[symmetric] in_these_eq .
         then have [simp]: "i' < k" by simp
 
         then have nth_i': "nth_or i' x xs = xs ! i'" if "length xs = k" for x :: 'x and xs
           unfolding nth_or_def \<open>length xs = k\<close> by (rule if_P)
         from \<open>i < k'\<close> have "i < length (tapes c')" unfolding l_tps' .
-        have r_nth_or: "reorder p (tapes c') tps ! i = nth_or i' (tapes c' ! i) tps" for tps
+        have r_nth_or: "reorder is (tapes c') tps ! i = nth_or i' (tapes c' ! i) tps" for tps
           unfolding reorder_nth[OF \<open>i < length (tapes c')\<close>] by simp
 
         have \<delta>\<^sub>w': "M'.\<delta>\<^sub>w ?q ?hds' i = \<delta>\<^sub>w (state c) (heads c) i'"
@@ -777,7 +780,72 @@ next
   finally show ?thesis .
 qed
 
-end \<comment> \<open>\<^locale>\<open>reorder_tapes\<close>\<close>
+corollary reorder_step':
+  fixes c c' :: "('q, 's) TM_config"
+  assumes "wf_config c"
+    and "length (tapes c') = k'"
+  shows "M'.step (reorder_config is (tapes c') c) = reorder_config is (tapes c') (step c)"
+  using \<open>wf_config c\<close> by (rule reorder_step) (simp add: \<open>length (tapes c') = k'\<close>)
+
+corollary reorder_steps:
+  fixes c c' :: "('q, 's) TM_config"
+  assumes wfc: "wf_config c"
+    and wfc': "length (tapes c') = k'"
+  shows "M'.steps n (reorder_config is (tapes c') c) = reorder_config is (tapes c') (steps n c)"
+    (is "M'.steps n (?rc c) = ?rc (steps n c)")
+proof (induction n)
+  case (Suc n)
+  from \<open>wf_config c\<close> have wfcs: "wf_config (steps n c)" by blast
+  show ?case unfolding funpow.simps comp_def Suc.IH reorder_step'[OF wfcs wfc'] ..
+qed \<comment> \<open>case \<open>n = 0\<close> by\<close> simp
+
+
+
+end \<comment> \<open>\<^locale>\<open>TM_reorder_tapes\<close>\<close>
+
+context TM
+begin
+
+
+definition reorder_tapes :: "nat option list \<Rightarrow> ('q, 's::finite) TM"
+  where "reorder_tapes is \<equiv> TM_reorder_tapes.M' M is"
+
+corollary reorder_tapes_steps:
+  fixes c c' :: "('q, 's) TM_config"
+  assumes "wf_config c"
+    and "length (tapes c') = length is"
+    and "Option.these (set is) = {0..<k}"
+  shows "TM.steps (reorder_tapes is) n (reorder_config is (tapes c') c) = reorder_config is (tapes c') (steps n c)"
+  unfolding reorder_tapes_def using assms
+  by (intro TM_reorder_tapes.reorder_steps) (unfold_locales)
+
+
+definition tape_offset :: "nat \<Rightarrow> nat \<Rightarrow> nat option list"
+  where "tape_offset a b \<equiv> None\<up>a @ (map Some [0..<k]) @ None\<up>b"
+
+lemma tape_offset_length[simp]: "length (tape_offset a b) = a + k + b"
+  unfolding tape_offset_def by simp
+
+lemma tape_offset_valid: "Option.these (set (tape_offset a b)) = {0..<k}"
+proof -
+  let ?o = "tape_offset a b"
+  have [simp]: "set ?o = set (None \<up> a) \<union> Some ` {0..<k} \<union> set (None \<up> b)"
+    unfolding tape_offset_def by force
+  have [simp]: "Option.these (set (None \<up> i)) = {}" for i by (induction i) auto
+  show "Option.these (set ?o) = {0..<k}" by simp
+qed
+
+lemma tape_offset_steps:
+  fixes c c' :: "('q, 's) TM_config"
+    and a b :: nat
+  defines "is \<equiv> tape_offset a b"
+  assumes "wf_config c"
+    and "length (tapes c') = length is"
+  shows "TM.steps (reorder_tapes is) n (reorder_config is (tapes c') c) = reorder_config is (tapes c') (steps n c)"
+  using assms tape_offset_valid unfolding reorder_tapes_def is_def
+  by (intro TM_reorder_tapes.reorder_steps) (unfold_locales)
+
+end
 
 
 subsubsection\<open>Running a TM Program\<close>
